\documentclass{scrartcl}

\usepackage{enumitem, mathtools, mdframed, prftree}

\begin{document}
\section*{Problem 4}
\begin{mdframed}
  Prove the following in the sequent calculus. You may use any rule
  given in the notes, including the derived rules.

  \begin{enumerate}[label=(\alph*)]
  \item \(q \Rightarrow (p \vee \neg p)\)
  \item \(q \Rightarrow (p \vee q)\)
  \item \((\neg p) \Rightarrow (p \Rightarrow q)\)
  \end{enumerate}
\end{mdframed}

\begin{enumerate}[label=(\alph*)]
\item \input{q-implies-p-or-not-p}
\item \input{q-implies-p-or-q}
\item \input{not-p-implies-p-implies-q}
\end{enumerate}
\end{document}
